get rid of irregular environments

HolBASimps.sml
@@ -70,10 +70,8 @@ val bir_SIMPLE_REWRS_imm = rewrites [
 val bir_SIMPLE_REWRS_env = rewrites [
   bir_var_name_def,
   bir_var_type_def,
-  bir_is_regular_env_def,
   bir_is_well_typed_env_empty,
-  bir_env_write_Irregular,
-  bir_env_write_Irregular_WrongVal
+  bir_env_write_WrongVal
 ];
 
 
